HoTT.thy
@@ -1,0 +1,15 @@
+(*  Title:  HoTT/HoTT.thy
+    Author: Josh Chen
+
+Load all the component modules for the HoTT logic.
+*)
+
+theory HoTT imports
+  HoTT_Base
+  Prod Sum
+
+begin
+
+\<comment> \<open>Maybe tactic setup can go in here?\<close>
+
+end
